SStructTT/SStruct/Erasure/Normalize.lean
@@ -7,57 +7,36 @@ variable {Srt : Type}
 
 lemma Erased.value_step {m n : Tm Srt} :
     Value m -> m ~>> n -> False := by
-  intro vl st
-  cases st with
-  | inl st =>
-    induction st
-    all_goals cases vl; try aesop
-  | inr st =>
-    induction st
-    all_goals cases vl; try aesop
-
-@[simp]def drop_count : Tm Srt -> Nat
-  | .var _ => 0
-  | .lam m _ => drop_count m
-  | .app m n => drop_count m + drop_count n
-  | .tup m n _ => drop_count m + drop_count n
-  | .prj m n => drop_count m + drop_count n
-  | .tt => 0
-  | .ff => 0
-  | .ite m n1 n2 => drop_count m + drop_count n1 + drop_count n2
-  | .rw m => drop_count m
-  | .drop m n => 1 + drop_count m + drop_count n
-  | .ptr _ => 0
-  | .null => 0
-
-def DropCount : Tm Srt -> Tm Srt -> Prop  :=
-  InvImage (. < .) drop_count
-
-lemma Step0.sub_drop : Subrelation (flip Step0) (@DropCount Srt) := by
-  intro m m' st; simp[DropCount,InvImage]; induction st
-  all_goals try (solve| aesop)
-
-lemma Step0.flip_wf : WellFounded (flip (@Step0 Srt)) := by
-  apply Subrelation.wf Step0.sub_drop
-  eta_reduce
-  apply InvImage.wf
-  apply Nat.lt_wfRel.wf
-
-theorem Erased.normalize0 {m' : Tm Srt} : SN Step0 m' := by
-  have ⟨h⟩ := @Step0.flip_wf Srt
-  apply SN.ofAcc (h m')
+  intro vl st; induction vl generalizing n
+  case lam =>
+    rcases st with ⟨rd, st⟩
+    rw[Red0.lam_inv rd] at st
+    cases st
+  case tup ihm ihn =>
+    rcases st with ⟨rd, st⟩
+    have ⟨_, _, _, rd1, rd2⟩ := Red0.tup_inv rd
+    subst_vars
+    cases st
+    case tup_M st => apply ihm (Step.intro rd1 st)
+    case tup_N st => apply ihn (Step.intro rd2 st)
+  case tt =>
+    rcases st with ⟨rd, st⟩
+    rw[Red0.tt_inv rd] at st
+    cases st
+  case ff =>
+    rcases st with ⟨rd, st⟩
+    rw[Red0.ff_inv rd] at st
+    cases st
+  case ptr =>
+    rcases st with ⟨rd, st⟩
+    rw[Red0.ptr_inv rd] at st
+    cases st
+  case null =>
+    rcases st with ⟨rd, st⟩
+    rw[Red0.null_inv rd] at st
+    cases st
 
 variable [ord : SrtOrder Srt]
-
-theorem Erased.normalize1 {A m : SStruct.Tm Srt} {m'} :
-    [] ;; [] ⊢ m ▷ m' : A -> SN Step1 m' := by
-  intro er
-  have sn := er.toDynamic.normalize
-  induction sn generalizing m'
-  case intro m h ih =>
-  constructor; intro n' st'
-  have ⟨n, st, ern⟩ := er.preservation1 st'
-  apply ih <;> assumption
 
 theorem Erased.normalize {A m : SStruct.Tm Srt} {m'} :
     [] ;; [] ⊢ m ▷ m' : A -> SN Step m' := by
@@ -66,56 +45,5 @@ theorem Erased.normalize {A m : SStruct.Tm Srt} {m'} :
   induction sn generalizing m'
   case intro m h ih =>
   constructor; intro n' st'
-  have ⟨n, st, ern⟩ := er.preservation st'
-  cases st with
-  | inl => aesop
-  | inr =>
-    subst_vars
-    apply ih <;> try assumption
-    sorry
-
--- theorem Erased.normalize {A m : SStruct.Tm Srt} {m'} :
---     [] ;; [] ⊢ m ▷ m' : A -> SN Step m' := by
---   intro er; unfold Step
---   apply Classical.byContradiction; intro nn
---   have := SN.negate nn
---   constructor
-
--- theorem Erased.normalize0 {m' : Tm Srt} : SN Step0 m' := by
---   induction m'
---   sorry
---   sorry
---   case app ihm ihn =>
---     replace ⟨ihm⟩ := ihm
---     replace ⟨ihn⟩ := ihn
---     constructor
---     apply Classical.byContradiction
---     intro h; simp at h
---     have ⟨x, st, nn⟩ := h
---     cases st
---     case a.h.app_M =>
-
---       sorry
---     case a.h.app_N =>
---       sorry
-
-
---     sorry
-
-
-  -- constructor
-  -- apply Classical.byContradiction; intro h
-  -- simp at h
-  -- induction m'
-  -- case a.h.var =>
-  --   have ⟨m, st, sn⟩ := h
-  --   cases st
-  -- case a.h.lam =>
-  --   have ⟨m, st, sn⟩ := h
-  --   cases st
-  -- case a.h.app ihm ihn =>
-  --   have ⟨m, st, sn⟩ := h
-  --   cases st
-  --   case app_M x st =>
-  --     sorry
-  --   case app_N => sorry
+  have ⟨n, st, ern⟩ := er.preservation1 st'
+  apply ih <;> assumption
